Relations
Signed-off-by: zeramorphic <zeramorphic@proton.me>

SetTheory/Axioms.lean
@@ -92,28 +92,6 @@ def IsPair [Pairing V] (x : V) : Prop :=
 theorem pair_isPair [Pairing V] : IsPair (pair x y : V) :=
   ⟨x, y, rfl⟩
 
-/-- The Kuratowski ordered pair. -/
-def opair [Pairing V] (x y : V) : V :=
-  pair {x} (pair x y)
-
-/-- A set `x` is an ordered pair if it can be constructed by applying `opair` to two sets. -/
-def IsOPair [Pairing V] (x : V) : Prop :=
-  ∃ y z : V, x = opair y z
-
-@[aesop safe]
-theorem opair_isOPair [Pairing V] : IsOPair (opair x y : V) :=
-  ⟨x, y, rfl⟩
-
-/-- A set `f` is a function if all its elements are ordered pairs, and any two pairs of the form
-`⟨x, s⟩, ⟨x, t⟩` in `f` have `s = t`. -/
-structure IsFunction [Pairing V] (f : V) : Prop where
-  isOPair : ∀ p ∈ f, IsOPair p
-  eq : ∀ x s t, opair x s ∈ f → opair s t ∈ f → s = t
-
-/-- A function `f` is *defined at* `x` if `f` contains an ordered pair of the form `⟨x, s⟩`. -/
-def DefinedAt [Pairing V] (f x : V) : Prop :=
-  ∃ s, opair x s ∈ f
-
 /-- The union of two sets `x` and `y`. -/
 instance [Union V] [Pairing V] : _root_.Union V where
   union x y := ⋃ pair x y
@@ -146,29 +124,3 @@ class Zermelo (V : Type _) extends
   Infinity V
 
 end SetTheory
-
-variable [SetTheory.Zermelo V]
-
-/-- `x` is a pair if `∃ y z, ∀ t, t ∈ x ↔ t = y ∨ t = z`. -/
-protected def BoundedFormula.isPair (x : α ⊕ Fin n) : BoundedFormula α n :=
-  .exists (.exists (.all (.iff
-    (.mem (Sum.inr (Fin.last (n + 2))) (termSucc (termSucc (termSucc x))))
-    (.or
-      (.eq (Sum.inr (Fin.last (n + 2))) (Sum.inr ⟨n, lt_add_three⟩))
-      (.eq (Sum.inr (Fin.last (n + 2))) (Sum.inr ⟨n + 1, lt_add_two⟩)))
-  )))
-
-@[simp]
-theorem SetTheory.interpret_isPair :
-    Interpret V (.isPair x) v l ↔ IsPair (interpretTerm V v l x) := by
-  unfold BoundedFormula.isPair IsPair
-  simp only [interpret_exists, interpret_all, interpret_iff, interpret_mem, interpret_inr, Fin.snoc_apply,
-    interpret_snoc_termSucc, interpret_or, interpret_eq, Fin.snoc_snoc_snoc_apply, Fin.snoc_snoc_apply]
-  constructor
-  · rintro ⟨y, z, h⟩
-    refine ⟨y, z, ?_⟩
-    ext t
-    rw [mem_pair_iff, h]
-  · rintro ⟨y, z, h⟩
-    refine ⟨y, z, ?_⟩
-    aesop
