SetTheory.lean
@@ -2,3 +2,6 @@ import SetTheory.SetTheory
 import SetTheory.Formula
 import SetTheory.Axioms
 import SetTheory.Basic
+import SetTheory.OPair
+import SetTheory.Relation
+import SetTheory.Function
