SetTheory/Function.lean
@@ -1,0 +1,12 @@
+import SetTheory.Relation
+
+namespace SetTheory
+
+variable [Zermelo V] {r x y z : V}
+
+/-- A set `f` is a function if all its elements are ordered pairs, and any two pairs of the form
+`⟨x, s⟩, ⟨x, t⟩` in `f` have `s = t`. -/
+structure IsFunction (f : V) extends IsRelation f : Prop where
+  eq : ∀ x s t, opair x s ∈ f → opair s t ∈ f → s = t
+
+end SetTheory
