SetTheory/OPair.lean
@@ -1,0 +1,188 @@
+import SetTheory.Basic
+
+namespace SetTheory
+
+variable [Zermelo V] {x y z : V}
+
+/-- The Kuratowski ordered pair. -/
+def opair [Pairing V] (x y : V) : V :=
+  pair {x} (pair x y)
+
+/-- A set `x` is an ordered pair if it can be constructed by applying `opair` to two sets. -/
+def IsOPair [Pairing V] (x : V) : Prop :=
+  ∃ y z : V, x = opair y z
+
+@[aesop safe]
+theorem opair_isOPair [Pairing V] : IsOPair (opair x y : V) :=
+  ⟨x, y, rfl⟩
+
+/-- The first projection of a Kuratowski ordered pair. -/
+def π₁ (x : V) : V :=
+  ⋃ ⋂ x
+
+/-- The second projection of a Kuratowski ordered pair. -/
+def π₂ (x : V) : V :=
+  ⋃ sep
+    (.imp
+      (.ne (Sum.inl true) (Sum.inl false))
+      (.not (.mem (Sum.inr 0) (Sum.inl false))))
+    (fun i => if i then ⋃ x else ⋂ x) (⋃ x)
+
+theorem mem_π₂_iff : y ∈ π₂ x ↔ ∃ z, y ∈ z ∧ z ∈ ⋃ x ∧ (⋃ x ≠ ⋂ x → z ∉ ⋂ x) := by
+  unfold π₂
+  aesop
+
+@[simp]
+theorem π₁_opair : π₁ (opair x y) = x := by
+  unfold π₁ opair
+  ext z
+  aesop
+
+@[simp]
+theorem π₂_opair : π₂ (opair x y) = y := by
+  unfold opair
+  ext z
+  rw [mem_π₂_iff]
+  simp only [sUnion_pair, sInter_pair, ne_eq, union_pair_eq_inter_pair]
+  constructor
+  · rintro ⟨s, hzs, hsx, hs⟩
+    by_cases h : s = y
+    · subst h
+      exact hzs
+    · aesop
+  · aesop
+
+@[simp]
+theorem opair_injective {x y z w : V} :
+    opair x y = opair z w ↔ x = z ∧ y = w := by
+  constructor
+  · intro h
+    have h₁ := congrArg π₁ h
+    have h₂ := congrArg π₂ h
+    simp at h₁ h₂
+    exact ⟨h₁, h₂⟩
+  · rintro ⟨rfl, rfl⟩
+    rfl
+
+/-- `x` is the pair `{y, z}` if `∀ t, t ∈ x ↔ t = y ∨ t = z`. -/
+protected def _root_.BoundedFormula.eqPair (x y z : α ⊕ Fin n) : BoundedFormula α n :=
+  .all (.iff
+    (.mem (Sum.inr (Fin.last n)) (termSucc x))
+    (.or
+      (.eq (Sum.inr (Fin.last n)) (termSucc y))
+      (.eq (Sum.inr (Fin.last n)) (termSucc z)))
+  )
+
+theorem eq_pair_iff : x = pair y z ↔ ∀ t, t ∈ x ↔ t = y ∨ t = z := by
+  rw [ext_iff]
+  simp
+
+@[simp]
+theorem interpret_eqPair {x y z : α ⊕ Fin n} :
+    Interpret V (.eqPair x y z) v l ↔
+      interpretTerm V v l x = pair (interpretTerm V v l y) (interpretTerm V v l z) := by
+  unfold BoundedFormula.eqPair
+  rw [eq_pair_iff]
+  simp
+
+/-- `x` is the singleton `{y}` if it is the pair `{y, y}`. -/
+protected def _root_.BoundedFormula.eqSingleton (x y : α ⊕ Fin n) : BoundedFormula α n :=
+  .eqPair x y y
+
+@[simp]
+theorem interpret_eqSingleton {x y : α ⊕ Fin n} :
+    Interpret V (.eqSingleton x y) v l ↔
+      interpretTerm V v l x = {interpretTerm V v l y} := by
+  unfold BoundedFormula.eqSingleton
+  simp
+
+/-- `x` is a pair if `∃ y z, ∀ t, t ∈ x ↔ t = y ∨ t = z`. -/
+protected def _root_.BoundedFormula.isPair (x : α ⊕ Fin n) : BoundedFormula α n :=
+  .exists (.exists (.eqPair
+    (termSucc (termSucc x))
+    (Sum.inr ⟨n, Nat.lt_add _⟩)
+    (Sum.inr (Fin.last (n + 1)))
+  ))
+
+@[simp]
+theorem interpret_isPair {x : α ⊕ Fin n} :
+    Interpret V (.isPair x) v l ↔ IsPair (interpretTerm V v l x) := by
+  unfold BoundedFormula.isPair IsPair
+  simp
+
+/-- `x` is the ordered pair `(y, z)` if `∃ y' z', y' = {y}, z' = {y, z}, x = {y', z'}`. -/
+protected def _root_.BoundedFormula.eqOPair (x y z : α ⊕ Fin n) : BoundedFormula α n :=
+  .exists (.exists (
+    .and (.and
+      (.eqSingleton (Sum.inr ⟨n, Nat.lt_add 1⟩) (termSucc (termSucc y)))
+      (.eqPair (Sum.inr ⟨n + 1, Nat.lt_add 0⟩)
+        (termSucc (termSucc y)) (termSucc (termSucc z))))
+      (.eqPair (termSucc (termSucc x))
+        (Sum.inr ⟨n, Nat.lt_add 1⟩) (Sum.inr ⟨n + 1, Nat.lt_add 0⟩))
+  ))
+
+@[simp]
+theorem interpret_eqOPair {x y z: α ⊕ Fin n} :
+    Interpret V (.eqOPair x y z) v l ↔
+    interpretTerm V v l x = opair (interpretTerm V v l y) (interpretTerm V v l z) := by
+  unfold BoundedFormula.eqOPair opair
+  aesop
+
+/-- `x` is a pair if `∃ y z, x = {{y}, {y, z}}`.
+More formally, we will write `∃ y z y' z', y' = {y}, z' = {y, z}, x = {y', z'}`. -/
+protected def _root_.BoundedFormula.isOPair (x : α ⊕ Fin n) : BoundedFormula α n :=
+  .exists (.exists (.eqOPair
+    (termSucc (termSucc x))
+    (Sum.inr ⟨n, Nat.lt_add 1⟩)
+    (Sum.inr ⟨n + 1, Nat.lt_add 0⟩)))
+
+@[simp]
+theorem interpret_isOPair {x : α ⊕ Fin n} :
+    Interpret V (.isOPair x) v l ↔ IsOPair (interpretTerm V v l x) := by
+  unfold BoundedFormula.isOPair IsOPair opair
+  aesop
+
+/-- `x` is an ordered pair in `y × z` if `∃ a ∈ y, ∃ b ∈ z, x = (a, b)`. -/
+protected def _root_.BoundedFormula.memProd (x y z : α ⊕ Fin n) : BoundedFormula α n :=
+  .exists (.exists (.and (.and
+    (.mem (Sum.inr ⟨n, Nat.lt_add 1⟩) (termSucc (termSucc y)))
+    (.mem (Sum.inr ⟨n + 1, Nat.lt_add 0⟩) (termSucc (termSucc z))))
+    (.eqOPair (termSucc (termSucc x))
+      (Sum.inr ⟨n, Nat.lt_add 1⟩) (Sum.inr ⟨n + 1, Nat.lt_add 0⟩))))
+
+theorem interpret_memProd' {x y z : α ⊕ Fin n} :
+    Interpret V (.memProd x y z) v l ↔
+    ∃ a ∈ interpretTerm V v l y, ∃ b ∈ interpretTerm V v l z, interpretTerm V v l x = opair a b := by
+  unfold BoundedFormula.memProd
+  aesop
+
+def prod (x y : V) : V :=
+  sep
+    (.memProd (Sum.inr 0) (Sum.inl true) (Sum.inl false))
+    (fun (i : Bool) => if i then x else y)
+    (power (power (x ∪ y)))
+
+theorem mem_prod_iff : z ∈ prod x y ↔ ∃ a ∈ x, ∃ b ∈ y, z = opair a b := by
+  unfold prod
+  simp only [mem_sep_iff, mem_power_iff, interpret_memProd', interpret_inl, ite_true,
+    ite_false, interpret_inr, and_iff_right_iff_imp, forall_exists_index, and_imp]
+  rintro a ha b hb rfl
+  intro z hz
+  rw [opair, mem_pair_iff] at hz
+  obtain (rfl | rfl) := hz <;>
+  · rw [mem_power_iff]
+    intro t ht
+    aesop
+
+@[simp]
+theorem opair_mem_prod_iff {a b : V} : opair a b ∈ prod x y ↔ a ∈ x ∧ b ∈ y := by
+  rw [mem_prod_iff]
+  aesop
+
+@[simp]
+theorem interpret_isOPairIn {x y z : α ⊕ Fin n} :
+    Interpret V (.memProd x y z) v l ↔
+    interpretTerm V v l x ∈ prod (interpretTerm V v l y) (interpretTerm V v l z) := by
+  rw [mem_prod_iff, interpret_memProd']
+
+end SetTheory
