SetTheory/Relation.lean
@@ -1,0 +1,294 @@
+import SetTheory.OPair
+
+namespace SetTheory
+
+variable [Zermelo V] {r x y z : V}
+
+structure IsRelation (r : V) : Prop where
+  isOPair : ∀ p ∈ r, IsOPair p
+
+theorem opair_left_mem_sUnion_sUnion (hxyr : opair x y ∈ r) :
+    x ∈ ⋃ ⋃ r := by
+  simp only [mem_sUnion_iff]
+  refine ⟨{x}, ⟨_, hxyr, ?_⟩, ?_⟩
+  · simp only [opair, mem_pair_iff, true_or]
+  · rw [mem_singleton_iff]
+
+theorem opair_right_mem_sUnion_sUnion (hxyr : opair x y ∈ r) :
+    y ∈ ⋃ ⋃ r := by
+  simp only [mem_sUnion_iff]
+  refine ⟨pair x y, ⟨_, hxyr, ?_⟩, ?_⟩
+  · simp only [opair, mem_pair_iff, or_true]
+  · exact right_mem_pair
+
+/-- `x` is in the domain of the relation `r` if `∃ z, (x, z) ∈ r`.
+More formally we write `∃ z t, t = (x, z), t ∈ r`. -/
+protected def _root_.BoundedFormula.memDom (x r : α ⊕ Fin n) : BoundedFormula α n :=
+  .exists (.exists (.and
+    (.eqOPair (Sum.inr ⟨n + 1, Nat.lt_add 0⟩) (termSucc (termSucc x)) (Sum.inr ⟨n, Nat.lt_add 1⟩))
+    (.mem (Sum.inr ⟨n + 1, Nat.lt_add 0⟩) (termSucc (termSucc r)))))
+
+theorem interpret_memDom' {x r : α ⊕ Fin n} :
+    Interpret V (.memDom x r) v l ↔
+    ∃ z, opair (interpretTerm V v l x) z ∈ interpretTerm V v l r := by
+  unfold BoundedFormula.memDom
+  simp
+
+def dom (r : V) : V :=
+  sep (.memDom (Sum.inr 0) (Sum.inl ())) (fun (_ : Unit) => r) (⋃ ⋃ r)
+
+theorem mem_dom_iff : x ∈ dom r ↔ ∃ z, opair x z ∈ r := by
+  unfold dom
+  simp only [mem_sep_iff, interpret_memDom', interpret_inr, interpret_inl,
+    and_iff_right_iff_imp, forall_exists_index]
+  intro t
+  exact opair_left_mem_sUnion_sUnion
+
+@[simp]
+theorem interpret_memDom {x r : α ⊕ Fin n} :
+    Interpret V (.memDom x r) v l ↔ interpretTerm V v l x ∈ dom (interpretTerm V v l r) := by
+  rw [mem_dom_iff, interpret_memDom']
+
+/-- `x` is in the range of the relation `r` if `∃ z, (z, x) ∈ r`.
+More formally we write `∃ z t, t = (z, x), t ∈ r`. -/
+protected def _root_.BoundedFormula.memRan (x r : α ⊕ Fin n) : BoundedFormula α n :=
+  .exists (.exists (.and
+    (.eqOPair (Sum.inr ⟨n + 1, Nat.lt_add 0⟩) (Sum.inr ⟨n, Nat.lt_add 1⟩) (termSucc (termSucc x)))
+    (.mem (Sum.inr ⟨n + 1, Nat.lt_add 0⟩) (termSucc (termSucc r)))))
+
+theorem interpret_memRan' {x r : α ⊕ Fin n} :
+    Interpret V (.memRan x r) v l ↔
+    ∃ z, opair z (interpretTerm V v l x) ∈ interpretTerm V v l r := by
+  unfold BoundedFormula.memRan
+  simp
+
+def ran (r : V) : V :=
+  sep (.memRan (Sum.inr 0) (Sum.inl ())) (fun (_ : Unit) => r) (⋃ ⋃ r)
+
+theorem mem_ran_iff : x ∈ ran r ↔ ∃ z, opair z x ∈ r := by
+  unfold ran
+  simp only [mem_sep_iff, interpret_memRan', interpret_inr, interpret_inl,
+    and_iff_right_iff_imp, forall_exists_index]
+  intro t
+  exact opair_right_mem_sUnion_sUnion
+
+@[simp]
+theorem interpret_memRan {x r : α ⊕ Fin n} :
+    Interpret V (.memRan x r) v l ↔ interpretTerm V v l x ∈ ran (interpretTerm V v l r) := by
+  rw [mem_ran_iff, interpret_memRan']
+
+/-- `x` is in the image of `y` under the relation `r` if `∃ z ∈ y, (z, x) ∈ r`. -/
+protected def _root_.BoundedFormula.memImage (x y r : α ⊕ Fin n) : BoundedFormula α n :=
+  .exists (.exists (.and (.and
+    (.mem (Sum.inr ⟨n, Nat.lt_add 1⟩) (termSucc (termSucc y)))
+    (.eqOPair (Sum.inr ⟨n + 1, Nat.lt_add 0⟩) (Sum.inr ⟨n, Nat.lt_add 1⟩) (termSucc (termSucc x))))
+    (.mem (Sum.inr ⟨n + 1, Nat.lt_add 0⟩) (termSucc (termSucc r)))))
+
+theorem interpret_memImage' {x y r : α ⊕ Fin n} :
+    Interpret V (.memImage x y r) v l ↔
+    ∃ z ∈ interpretTerm V v l y, opair z (interpretTerm V v l x) ∈ interpretTerm V v l r := by
+  unfold BoundedFormula.memImage
+  aesop
+
+def image (r y : V) : V :=
+  sep
+    (.memImage (Sum.inr 0) (Sum.inl false) (Sum.inl true))
+    (fun (i : Bool) => if i then r else y)
+    (ran r)
+
+theorem mem_image_iff : x ∈ image r y ↔ ∃ z ∈ y, opair z x ∈ r := by
+  unfold image
+  simp only [mem_sep_iff, mem_ran_iff, interpret_memImage']
+  aesop
+
+@[simp]
+theorem interpret_memImage {x y r : α ⊕ Fin n} :
+    Interpret V (.memImage x y r) v l ↔
+    interpretTerm V v l x ∈ image (interpretTerm V v l r) (interpretTerm V v l y) := by
+  rw [mem_image_iff, interpret_memImage']
+
+/-- `x` is in the preimage of `y` under the relation `r` if `∃ z ∈ y, (x, z) ∈ r`. -/
+protected def _root_.BoundedFormula.memPreimage (x y r : α ⊕ Fin n) : BoundedFormula α n :=
+  .exists (.exists (.and (.and
+    (.mem (Sum.inr ⟨n, Nat.lt_add 1⟩) (termSucc (termSucc y)))
+    (.eqOPair (Sum.inr ⟨n + 1, Nat.lt_add 0⟩) (termSucc (termSucc x)) (Sum.inr ⟨n, Nat.lt_add 1⟩)))
+    (.mem (Sum.inr ⟨n + 1, Nat.lt_add 0⟩) (termSucc (termSucc r)))))
+
+theorem interpret_memPreimage' {x y r : α ⊕ Fin n} :
+    Interpret V (.memPreimage x y r) v l ↔
+    ∃ z ∈ interpretTerm V v l y, opair (interpretTerm V v l x) z ∈ interpretTerm V v l r := by
+  unfold BoundedFormula.memPreimage
+  aesop
+
+def preimage (r y : V) : V :=
+  sep
+    (.memPreimage (Sum.inr 0) (Sum.inl false) (Sum.inl true))
+    (fun (i : Bool) => if i then r else y)
+    (dom r)
+
+theorem mem_preimage_iff : x ∈ preimage r y ↔ ∃ z ∈ y, opair x z ∈ r := by
+  unfold preimage
+  simp only [mem_sep_iff, mem_dom_iff, interpret_memPreimage']
+  aesop
+
+@[simp]
+theorem interpret_memPreimage {x y r : α ⊕ Fin n} :
+    Interpret V (.memPreimage x y r) v l ↔
+    interpretTerm V v l x ∈ preimage (interpretTerm V v l r) (interpretTerm V v l y) := by
+  rw [mem_preimage_iff, interpret_memPreimage']
+
+/-- `x` is in the inverse of the relation `r` if `x = (y, z)` and `(z, y) ∈ r`. -/
+protected def _root_.BoundedFormula.memInverse (x r : α ⊕ Fin n) : BoundedFormula α n :=
+  -- ∃ y z t
+  .exists (.exists (.exists (.and (.and
+    -- x = (y, z)
+    (.eqOPair (termSucc (termSucc (termSucc x)))
+      (Sum.inr ⟨n, Nat.lt_add 2⟩) (Sum.inr ⟨n + 1, Nat.lt_add 1⟩))
+    -- t = (z, y)
+    (.eqOPair (Sum.inr ⟨n + 2, Nat.lt_add 0⟩)
+      (Sum.inr ⟨n + 1, Nat.lt_add 1⟩) (Sum.inr ⟨n, Nat.lt_add 2⟩)))
+    -- t ∈ r
+    (.mem (Sum.inr ⟨n + 2, Nat.lt_add 0⟩) (termSucc (termSucc (termSucc r)))))))
+
+theorem interpret_memInverse' {x r : α ⊕ Fin n} :
+    Interpret V (.memInverse x r) v l ↔
+    ∃ y z, interpretTerm V v l x = opair y z ∧ opair z y ∈ interpretTerm V v l r := by
+  unfold BoundedFormula.memInverse
+  aesop
+
+def inverse (r : V) : V :=
+  sep
+    (.memInverse (Sum.inr 0) (Sum.inl ()))
+    (fun (_ : Unit) => r)
+    (prod (ran r) (dom r))
+
+theorem mem_inverse_iff : x ∈ inverse r ↔ ∃ y z, x = opair y z ∧ opair z y ∈ r := by
+  unfold inverse
+  simp only [mem_sep_iff, interpret_memInverse']
+  constructor
+  · aesop
+  · rintro ⟨a, b, rfl, ha⟩
+    refine ⟨?_, by aesop⟩
+    rw [mem_prod_iff]
+    refine ⟨a, ?_, b, ?_, rfl⟩
+    · rw [mem_ran_iff]
+      exact ⟨b, ha⟩
+    · rw [mem_dom_iff]
+      exact ⟨a, ha⟩
+
+@[simp]
+theorem interpret_memInverse {x r : α ⊕ Fin n} :
+    Interpret V (.memInverse x r) v l ↔
+    interpretTerm V v l x ∈ inverse (interpretTerm V v l r) := by
+  rw [mem_inverse_iff, interpret_memInverse']
+
+@[aesop norm]
+theorem inverse_inverse (hr : IsRelation r) : inverse (inverse r) = r := by
+  ext x
+  simp only [mem_inverse_iff]
+  constructor
+  · aesop
+  · intro h
+    obtain ⟨y, z, rfl⟩ := hr.isOPair x h
+    exact ⟨y, z, rfl, z, y, rfl, h⟩
+
+@[simp]
+theorem image_inverse : image (inverse r) x = preimage r x := by
+  ext y
+  simp only [mem_image_iff, mem_preimage_iff, mem_inverse_iff]
+  aesop
+
+@[simp]
+theorem preimage_inverse : preimage (inverse r) x = image r x := by
+  ext y
+  simp only [mem_image_iff, mem_preimage_iff, mem_inverse_iff]
+  aesop
+
+/-- `x` is in the composition of the relations `s` and `r` if
+`∃ a b c, x = (a, c) ∧ (b, c) ∈ s ∧ (a, b) ∈ r`. -/
+protected def _root_.BoundedFormula.memComp (x s r : α ⊕ Fin n) : BoundedFormula α n :=
+  -- ∃ a b c d e
+  .exists (.exists (.exists (.exists (.exists (.and (.and (.and (.and
+    -- x = (a, c)
+    (.eqOPair (termSucc (termSucc (termSucc (termSucc (termSucc x)))))
+      (Sum.inr ⟨n, Nat.lt_add 4⟩) (Sum.inr ⟨n + 2, Nat.lt_add 2⟩))
+    -- d = (a, b)
+    (.eqOPair (Sum.inr ⟨n + 3, Nat.lt_add 1⟩)
+      (Sum.inr ⟨n, Nat.lt_add 4⟩) (Sum.inr ⟨n + 1, Nat.lt_add 3⟩)))
+    -- e = (b, c)
+    (.eqOPair (Sum.inr ⟨n + 4, Nat.lt_add 0⟩)
+      (Sum.inr ⟨n + 1, Nat.lt_add 3⟩) (Sum.inr ⟨n + 2, Nat.lt_add 2⟩)))
+    -- e ∈ s
+    (.mem (Sum.inr ⟨n + 4, Nat.lt_add 0⟩)
+      (termSucc (termSucc (termSucc (termSucc (termSucc s)))))))
+    -- d ∈ r
+    (.mem (Sum.inr ⟨n + 3, Nat.lt_add 1⟩)
+      (termSucc (termSucc (termSucc (termSucc (termSucc r)))))))))))
+
+theorem interpret_memComp' {x s r : α ⊕ Fin n} :
+    Interpret V (.memComp x s r) v l ↔
+    ∃ a b c,
+      interpretTerm V v l x = opair a c ∧
+      opair b c ∈ interpretTerm V v l s ∧
+      opair a b ∈ interpretTerm V v l r := by
+  unfold BoundedFormula.memComp
+  simp [and_assoc]
+
+def comp (s r : V) : V :=
+  sep
+    (.memComp (Sum.inr 0) (Sum.inl true) (Sum.inl false))
+    (fun (i : Bool) => if i then s else r)
+    (prod (dom r) (ran s))
+
+theorem mem_comp_iff : x ∈ comp s r ↔ ∃ a b c, x = opair a c ∧ opair b c ∈ s ∧ opair a b ∈ r := by
+  unfold comp
+  simp only [mem_sep_iff, interpret_memComp', interpret_inr, interpret_inl, ite_true, ite_false,
+    and_iff_right_iff_imp, forall_exists_index, and_imp]
+  rintro a b c rfl hs hr
+  rw [mem_prod_iff]
+  refine ⟨a, ?_, c, ?_, rfl⟩
+  · rw [mem_dom_iff]
+    exact ⟨b, hr⟩
+  · rw [mem_ran_iff]
+    exact ⟨b, hs⟩
+
+theorem interpret_memComp {x s r : α ⊕ Fin n} :
+    Interpret V (.memComp x s r) v l ↔
+    interpretTerm V v l x ∈ comp (interpretTerm V v l s) (interpretTerm V v l r) := by
+  rw [mem_comp_iff, interpret_memComp']
+
+theorem comp_assoc : comp (comp t s) r = comp t (comp s r) := by
+  ext
+  simp only [mem_comp_iff]
+  aesop
+
+/-- `x` is a member of the identity relation on `y` if `∃ z ∈ y, x = (z, z)`. -/
+protected def _root_.BoundedFormula.memId (x y : α ⊕ Fin n) : BoundedFormula α n :=
+  .exists (.and
+    (.mem (Sum.inr (Fin.last n)) (termSucc y))
+    (.eqOPair (termSucc x) (Sum.inr (Fin.last n)) (Sum.inr (Fin.last n))))
+
+theorem interpret_memId' {x y : α ⊕ Fin n} :
+    Interpret V (.memId x y) v l ↔
+    ∃ z ∈ interpretTerm V v l y, interpretTerm V v l x = opair z z := by
+  unfold BoundedFormula.memId
+  simp
+
+def id (x : V) : V :=
+  sep
+    (.memId (Sum.inr 0) (Sum.inl ()))
+    (fun (_ : Unit) => x)
+    (prod x x)
+
+theorem mem_id_iff : y ∈ id x ↔ ∃ z ∈ x, y = opair z z := by
+  unfold id
+  simp only [mem_sep_iff, interpret_memId']
+  aesop
+
+@[simp]
+theorem interpret_memId {x y : α ⊕ Fin n} :
+    Interpret V (.memId x y) v l ↔
+    interpretTerm V v l x ∈ id (interpretTerm V v l y) := by
+  rw [mem_id_iff, interpret_memId']
+
+end SetTheory
